
   \magnification=1200
   \baselineskip 14 pt
%  21 November 2012.
%I began this file on the base of the previous file caonisomorph1.tex

\def\V {{\cal V}}
\def\s {{\sigma}}
\def\Q {{\bf Q}}
\def\D {{\cal D}}
\def\G {{\Gamma}}
\def\C {{\bf C}}
\def\M {{\cal M}}
\def\Z {{\bf Z}}
\def\U  {{\cal U}}
\def\H {{\cal H}}
\def\R  {{\bf R}}
\def\l {\lambda}
\def\w {\omega}
\def\p {\partial}
\def\r {{\bf r}}
\def\v {{\bf v}}
\def\n {{\bf n}}
\def\t  {\tilde}
\def\b {{\bf b}}
\def\ac {{\bf a}}
\def \X   {{\bf X}}
\def \Y   {{\bf Y}}
\def \E   {{\bf E}}
\def \N   {{\bf N}}


\centerline {\bf On canonical isomorphisms $T^*E=T^*E^*$ for vector bundle $E$}


   \centerline{${\cal x}0$}

  Kirill Mackenzie told and explained many many times the construction of
remarkable isomorphism between cotangent bundles of 
vector bundle and its dual: for an arbitrary vector bundle $E$
                  $$
               T^*E=T^*E^*\,,
      \eqno(0.1)
                  $$
where $E^*$ is a bundle dula to $E$.

The first thing that you try to apply this constrution to it is to consider
  tangent bundle: $E=TM$ or cotangent bundle $E=T^*M$ and consider  
  isomorphism
              $$
          T^*TM=T^*T^*M
                       \eqno (0.2)
               $$
On the other hand in this special case
the canonical symplecctic structure on the cotangent bundle $T^*M$ implies
the canonical isomorphism between tangent and cotangent bundles of
the manifold $T^*M$:
              $$
         T^*T^*M=TT^*M
         \eqno (0.3)
             $$
Hence in the special case of $E=TM$ the ''Mackenzie'' isomorphism 
 (0.1) induces the canonical isomorphisms:
              $$
         T^*T^*M=T^*TM=TT^*M\,.
         \eqno (0.4)
             $$
In particual we see that in this case there is a 
canonical isomorphism
              $$
         T^*TM=TT^*M\,.
         \eqno (0.5)
             $$

In this etude we would like to reconstruct 
the ''Mackenzie'' isomorphism (0.1) and its special case the isomorphisms
(0.4) and (0.5) using pedestrian's arguments.  
 In the first section we conisder the special case
$E=TM$ and establish the isomorphisms (0.5) and (0.4)

Our notations are little bit inconsistent: in the first paragraph we
denote indices of coordinates by latin letters $i,j,k$ and new ones by
 greek letters. In the second paragraph our notations are much more traditional:
indices of new coordinates are denoted by the same letters with ''prime'' indices
  ($x^i\to x^{i'}$). 
\medskip

\centerline{ \bf Canonical isomorphism $TT^*M=T^*TM$}

  Let $M$ be manifold. Establish and study canonical isomorphisms $TT^*M=T^*TM=T^*T^*M$.

   Perform calculations in local coordinates.
It may sounds surprising but calculations in local coordinates are transparent and illuminating.


 First consider local coordinates on $TM$ and $T^*M$ corresponding to
local coordinates $(x^i)$ on $M$.
 Local coordinates for $TM$ are $(x^i,t^j)$: every vector $\r\in TM$ is a vector
  $t^i{\p\over \p x^i}$, $t^i(\r)=dx^i(\r)$.
         If   $\tilde x^\mu=\tilde x^\mu(x^i)$  are new local coordinates  on $M$
then
                  $$
            d\t x^\mu\left(t^i{\p\over \p x^i}\right)={\p \tilde x^\mu(x^i)\over \p x^i}dx^i
            \left(t^i{\p\over \p x^i}\right)={\p \tilde x^\mu(x^i)\over \p x^i}t^i\,.
              \eqno(1.1)
                  $$
Hence changing of local coordinates in $TM$ is
                    $$
                    (x^i,t^j)\mapsto (\t x^\mu, \t t^\nu),\quad \t x^\mu=\t x^\mu(x^i),\,\,
                 \tilde t^\mu=\pmatrix{\mu\cr i\cr}t^i,
                 \eqno(1.2)
                    $$
where we denote ${\p \tilde x^\mu(x^i)\over \p x^i}$ by  $\pmatrix{\mu\cr i\cr}$.



  Respectively local coordinates for $T^*M$ are $(x^i,p_j)$. For every $1$-form $\w\in T^*M$
  $p_i=\w\left({\p\over \p x^i}\right)$. Under changing of local coordinates on $M$
             $\tilde x^\mu=\tilde x^\mu(x^i)$, coordinates $(p_i)$ change to new coordinates $(p_\mu)$:
                           $$
p_\mu=w\left({\p\over \p \t x^\mu}\right)=
\w\left({\p x^i(\tilde x^\mu)\over \p \tilde x^\mu }
{\p\over \p  x^i}\right)={\p x^i(\tilde x^\mu)\over \p \tilde x^\mu }p_i
                           $$
Hence changing of local coordinates in $T^*M$ is
                        $$
                        (x^i,p_k)\mapsto (\tilde x^\mu,\tilde p_\nu),
                        \quad \t x^\mu=\t x^\mu(x^i),\,\,
                           p_\mu=\pmatrix{i\cr \mu\cr}p_i,
                           \eqno (2)
                        $$
where we denote ${\p x^i(\tilde x^\mu)\over \p \tilde x^\mu }$ by  $\pmatrix{i\cr \mu\cr}$


  Now using (1),(2) we define coordinates on the spaces
$TT^*M$, $T^*TM$ and $T^*T^*M$.


The space  $TT^*M$ is tangent space to the space $T^*M$. The local coordinates on $TT^*M$
corresponding to local coordinates $(x^i,p_j)$
on $T^*M$ are coordinates $(x^i,p_j;\xi^k,\rho_m)$; $\xi^k=dx^i(\r),\rho_m=dp_m(\r)$.
Under changing of local coordinates  $(x^i)$ to coordinates $\t x^\mu=\tilde x^\mu(x^i)$
coordinates $(\xi^i)$ and $(\rho_m)$ transform to new coordinates $(\t \xi^\mu)$ and $(\t \rho_\nu)$ respectively.
It follows from (1) that
                       $$
                    \t\xi^\mu={\p \t x^\mu\over \p x^i}\xi^i+{\p \t x^\mu\over \p p_i}\rho_i=\pmatrix{\mu\cr i\cr}\xi^i
                    \eqno (3)
                       $$
  because  ${\p \t x^\mu\over \p p_i}=0$.
  For transformation of coordinates $(\rho_m)$ calculations are longer:
            $$
  \t\rho_\mu={\p \t p_\mu\over \p x^i}\xi^i+{\p \t p_\mu\over \p p_i}\rho_i
            $$
We see that   ${\p \t p_\mu\over \p p_i}={\p\over \p p_i}
\left(\t p_\mu=\pmatrix {k\cr \mu\cr}p_k\right)=\pmatrix {i\cr \mu\cr}$ and
                           $$
{\p \t p_\mu\over \p x^i}={\p\over \p x^i}\left(\t p_\mu=\pmatrix {k\cr \mu\cr}p_k\right)=
 \pmatrix {\nu\cr i\cr} \pmatrix {k\cr\nu \mu\cr}p_k,
                           $$
where we denote as always by  $\pmatrix {\nu\cr i\cr}$ the partial derivative ${\p \t x^\mu\over \p x^i}$
and by $\pmatrix {k\cr\nu \mu\cr}$ the partial derivative ${\p^2 x^k\over \p \t x^\nu \p \t x^\mu}$.
The summation over repeated indices is assumed.  Finally we come to
                  $$
  \t\rho_\mu={\p \t p_\mu\over \p x^i}\xi^i+{\p \t p_\mu\over \p p_i}\rho_i=
  \xi^i\pmatrix {\nu\cr i\cr} \pmatrix {k\cr\nu \mu\cr}p_k+\pmatrix {i\cr \mu\cr}\rho_i
  \eqno (4)
                  $$


     Summarising:

    {\bf Proposition 1} {\it To local coordinates $(x^i)$ on $M$
    one can naturally assign local coordinates on $TT^*M$  $(x^i,p_j;\xi^k,\rho_m)$ such that
    under changing of coordinates $(x^i)\mapsto (\t x^\mu)$ on $M$ these coordinates transform in the following way}
                                $$
            \t p_\mu=\pmatrix{j\cr\mu\cr}p_j, \quad
            \t\xi^\mu=\pmatrix{\mu\cr i\cr}\xi^i,\quad
            \t\rho_\mu=
            \xi^i\pmatrix {\nu\cr i\cr} \pmatrix {k\cr\nu \mu\cr}p_k+\pmatrix {i\cr \mu\cr}\rho_i
            \eqno (*)
                                $$
\bigskip
Now consider coordinates  on $T^*TM$ and their transformation rules.
 If $(x,t)$ coordinates on $TM$ (see (1)) and $(x,t,\pi,\tau)$ corresponding coordinates on $T^*TM$
 ($\pi_k=\w\left({\p\over \p x^k}\right)$,
 $\tau_m=\w\left({\p\over \p t^m}\right)$) then according to (2)
 under changing of coordinates $(x^i)\mapsto (\t x^\mu)$, the coordinates $(\pi_m)$ transform to coordinates
 $(\t \pi_\mu)$, the coordinates $(\tau_k)$ transform to coordinates
 $(\t \tau_\nu)$ such that
                  $$
\t\pi_\mu={\p x^i\over \p \t x^\mu}\pi_i+{\p t^k\over \p \t x^\mu}\tau_k,\,\,\,\,
\t\tau_\nu={\p x^i\over \p \t t^\nu}\pi_i+{\p t^k\over \p \t t^\nu}\tau_k
                  $$
Since ${\p x^i\over \p \t t^\nu}=0$
and  ${\p t^k\over \p \t t^\nu}={\p x^k\over \p \t x^\mu}$
then $$\t\tau_\nu=\pmatrix {k\cr\nu}\tau_k$$.  For $\t\pi_\mu$ we have
                  $$
\t\pi_\mu=\pmatrix {i\cr\mu}\pi_i+{\p\over \p \t x^\mu}\left({\p x^k\over \p\t x^\nu}t^\nu\right)\tau_k=
\pmatrix {i\cr\mu}\pi_i+\pmatrix {k\cr\mu\nu}\pmatrix {\nu\cr i}t^i\tau_k\,.
                  $$

     Summarising:

    {\bf Proposition 2} {\it To local coordinates $(x^i)$ on $M$
    one can naturally assign local coordinates on $T^*TM$  $(x^i,t^j;\pi_k,\tau_j)$ such that
    under changing of coordinates $(x^i)\mapsto (\t x^\mu)$ on $M$ these coordinates transform in the following way}
                                $$
            \t \tau_\mu=\pmatrix{j\cr\mu\cr}\tau_j, \quad
            \t t^\mu=\pmatrix{\mu\cr i\cr}t^i,\quad
            \t\pi_\mu=
            t^i\pmatrix {\nu\cr i\cr} \pmatrix {k\cr\nu \mu\cr}\tau_k+\pmatrix {i\cr \mu\cr}\pi_i
            \eqno (**)
                                $$


Comparing  Propositions 1 and 2 we come to 

{\bf Observation 1}


Let $(x^i,t^i)$ be local coordinates on $TM$ and respectively $(x^i,p_i)$ be local coordinates on $T^*M$.
  Respectively one can consider local coordinates $(x^i,t^i;\pi_k,\tau_j)$ on $T^*TM$
 and $(x^i,p_i;\xi^k,\rho_m)$ on $T^*TM$. The map
                         $$
           t^i=\xi^i,\,\,\, \tau_j=p_j,\,\,\, \pi_k=\rho_k
                      \eqno (1.*)
                      $$
             establishes isomorphism between the spaces $T^*TM$ and $TT^*M$ which does not depend on
             the choice of local coordinates\footnote{$^*$}
{In fact one can consider the {\it pencil}  of maps 
          $$
 t^i={\ac}\xi^i,\,\,\, \tau_j={\bf b}p_j,\,\,\, \pi_k={\bf ab}\rho_k
\eqno ({\rm footnote})
             $$
where ${\bf a,b}\not=0$.}.


   Note canonical symplectic structure
$\Omega dp_i\wedge dx^i$ establishes isomorphism  between spaces $TT^*M$ and $T^*T^*M$: 
if $(x^i,p_i; r_m,\kappa^r))$ are local coordiantes on $T^*TM$ then this isomorphism looks like
             $$
 \rho_m=r_m,\xi^i=-\kappa_i,
\eqno (1.**)
             $$
Combining with isomorphism (1.*) we see that isomoprphism $T^*TM=T^*T^*M$ looks like
                            $$
            (x^i,t^i,\pi_k,-p_i)\leftrightarrow (x^i,p_i;\pi_k,t^i)
               \eqno (1.***)
                            $$ 
Of course there is two-parametric freedom related with (footnote).

\medskip

\centerline  {${\cal x}2 $ \bf Canoncial isomorphism in general case: $T^*E=T^*E$ }


 In the previous paragraph we constructed canonical isomorphism $T^*E=T^*E$ in the case where vector bundle $E$ is tangent (cotangent bundle).

  Now cosndier general case. Let $(x^\mu,s^i)$ be local coordiantes on bundle $E$.  Under changing of coordinates
   $x^{\mu'}=x^{\mu'}(x)$ fibre coordiantes $s^i$ transform in the following way:
                                     $$
                         s^{i'}=\Psi^{i'}_k(x)s^k\,.
                                     $$
Respectively dual fibre coordinates $s_k$ transform as:
                       $$
                 s_{k'}=\Phi_{k'}^is_i\,,
                       $$

where matrices $\Psi$ and $\Phi$ are inverse to each other: $\Psi^{i'}_k\Phi^k_{j'}=\delta^{i'}_{j'}$.

 Let $(x^\mu,s^i; \rho_\mu,\pi_i)$ be local coordinates in $T^*E$ and respectively
    let $(x^\mu,s_i; \zeta_\mu,t^i)$ be local coordinates in $T^*E^*$. Reccall that as usual we say that 
if $\w\in T^*E$ is $1$-form with  local coordinates $(x^\mu,s^i;\rho_\mu,\pi_i)$ if it is the function
on vectors tangent to the manifold $E$ at the point $(x^\mu, s^i)$ such that
              $$
     \w\left({\p\over \p x^\mu}\right) =\rho_\mu,\quad 
        \w\left({\p\over \p s^i}\right)=\pi_i
             $$
  Respectively we say that 
$\w\in T^*E^*$ is $1$-form with  coordinates $(x^\mu,s_i;\zeta_\mu,t_i)$ if it is the function
on vectors tangent to the manifold $E^*$ at the point $(x^\mu, s_i)$ such that
              $$
     \w\left({\p\over \p x^\mu}\right)=\zeta_\mu, \quad \w\left({\p\over \p s_i}\right)=t_i\,.
             $$
Write down transformation for fields under coordiante trasnformation $x^{\mu'}=x^{\mu'}(x^\mu)$. We have
                    $$
                   \cases
                    {
               s^{i'}=\Psi^{i'}_k(x)s^k\cr
            \rho_{\mu'}={\p x^\mu\over \p x^{\mu'}}\rho_\mu+
           {\p s^i\over\p x^{\mu'}}\pi_i\cr
                   \pi_{i'}={\p x^\mu\over \p s^{i'}}\rho_\mu+
       {\p s^i\over \p s^{i'}}\pi_i\cr
                      },\qquad
                    \cases
                    {
               s_{i'}=\Phi_{i'}^k(x)s_k\cr
 \zeta_{\mu'}={\p x^\mu\over \p x^{\mu'}}\zeta_\mu+
   {\p s_i\over\p x^{\mu'}}t^i \cr
    t^{i'}={\p x^\mu\over \p s_{i'}}\zeta_\mu+
  {\p s_i\over \p s_{i'}}t^i\cr
                      }
\eqno (2.1)
                      $$
Note that
                     $$
    {\p x^\mu\over \p s^{i'}}={\p x^\mu\over \p x^{\mu'}}=0,\,\,  {\p s^i\over \p s^{i'}}=\Phi^i_{i'},\,\,
    {\p s_i\over \p s_{i'}}=\Psi^{i'}_i\,,     
                     $$
and
                    $$
{\p s^i\over \p x^{\mu'}}\pi_i={\p \Phi^i_{i'}\over \p x^{\mu'}}s^{i'}\pi_i=
   {\p x^\mu\over \p x^{\mu'}}{\p \Phi^i_{i'}\over \p x^{\mu}}s^{i'}\pi_i=
   {\p x^\mu\over \p x^{\mu'}}
     {\p \Phi^i_{i'}\over \p x^{\mu}}
        \Psi^{i'}_ks^{k}\pi_i\,,
             \eqno (2.2a)
                   $$
                  $$
{\p s_i\over \p x^{\mu'}}t^i=
 {\p \Psi_i^{i'}\over \p x^{\mu'}}s_{i'}t^i=
   {\p x^\mu\over \p x^{\mu'}}{\p \Psi_i^{i'}\over \p x^{\mu}}
         s_{i'}t^i=
   {\p x^\mu\over \p x^{\mu}}{\p \Psi_i^{i'}\over \p x^{\mu}}
        \Phi_{i'}^ks_{k}t^i\,,
             \eqno (2.2b)
                   $$
Introducing  $L_{\mu k}^i$ such that
                 $$
         L_{\mu k}^i=
       {\p \Psi_k^{i'}\over \p x^{\mu}}
        \Phi_{i'}^i=
            -
       {\p \Phi^i_{i'}\over \p x^{\mu}}
        \Psi^{i'}_k=
             ,\,\,  \hbox 
        {since $\Psi\circ \Phi=1$}
                 $$
 
we see that the 
transformations (2.1) have the following appearance:
                   $$
                   \cases
                    {
               s^{i'}=\Psi^{i'}_k(x)s^k\cr
            \rho_{\mu'}={\p x^\mu\over \p x^{\mu'}}
                     \left(
                      \rho_\mu-
                     L_{\mu k}^is^k\pi_i
                      \right)
                      \cr
                   \pi_{i'}=\Phi^i_{i'}\pi_i\cr
                      },
                    \qquad
                    \cases
                    {
               s_{i'}=\Phi_{i'}^k(x)s_k\cr
 \zeta_{\mu'}={\p x^\mu\over \p x^{\mu'}}
        \left(
           \zeta_\mu+
               L_{\mu k}^it^k s_i
               \right)\cr
    t^{i'}=\Psi^{i'}_it^i\cr
                      }
\eqno (2.3)
                      $$
Put
         $$
       \cases
         {
      \pi_i=\alpha s_i\cr
      t^i=\beta s^i\cr
      \zeta_\mu=\gamma \rho_\mu\cr
        }
         $$
  We see that this map is invariant with respect to changing of coordinates
if $\beta=-\gamma\alpha$. In particular we can put $\alpha=-1$, $\beta=\gamma=1$
We come to isomorphism $T^*E=T^*E^*$ defined in local coordinates by condition
that
             $$
    (x^\mu,s^i;\rho_\mu,\pi_i)\leftrightarrow(x^\mu,s_i;\zeta_\mu,t^i),
   \quad\hbox{such that}\,\,\rho_\mu=\zeta_\mu,
      \pi_i=-s_i,t^i=s^i
             $$ 
(Compare with (1.***))
\bye
