


 \def\p{\partial}
\def\t {\tilde}
\def \m {\medskip}
\def\degree {{\bf {\rm degree}\,\,}}
\def \finish {${\,\,\vrule height1mm depth2mm width 8pt}$}





\def\a {\alpha}
\def\vare{{\varepsilon}}
\def\l {\lambda}
\def\s {{\sigma}}

\def\G {{\Gamma}}

\def\A {{\bf A}}
\def\C {{\bf C}}
\def\E  {{\bf E}}
\def\K {{\bf K}}
\def\N {{\bf N}}
\def\Q {{\bf Q}}
\def\R  {{\bf R}}
\def\V {{\cal V}}
\def \X   {{\bf X}}
\def \Y   {{\bf Y}}
\def\Z {{\bf Z}}



\def\ac {{\bf a}}
\def\e{{\bf e}}
\def\f {{\bf f}}
\def\n {{\bf n}}
\def\r {{\bf r}}
\def\v {{\bf v}}
\def \x   {{\bf x}}
\def \y   {{\bf y}}


\def\pt {{\bf pt}}



\centerline {\bf On one integral}


 Let $A(t)$ be a function on $\R$ such that
        $$
   A(t)=\sum_{k\geq l}\Psi_k t^k
      \eqno(1)
        $$
in a vicinity of $0$ and  $\int t^n A(t)dt$ converges at infinity for 
any $n$.

 Consider a function 
               $$
\zeta_A(s)={1\over G(s)}\int_0^\infty t^{s-1}A(t)dt,
           $$
where $\G(s)$ is the usual Gamma-function.
  This integral is well-defined for enough big $s$.

  Perform analytical prolongation and
calculate the derivative of the function $\zeta_A$ at the point $s=0$:
         $$
\zeta'_A(0)={d\over ds}\zeta_A(s)\big\vert_{s=0}=
   \sum_{k\not=0}{\Psi_k\over k}+
C\Psi_0+\int_1^\infty A(t){dt\over t}\,,
{\rm where}\,\,
    C=-\G'(1)\,.
       $$
  Statement:
        $$
   \zeta'_A(0)=
\int_0^\infty
     \left(
     A(t)-\sum_{k<0}\Psi_kt^k-e^{-t}\Psi_0
      \right)
     {dt\over t}\,.
     \eqno (2)
       $$
{\sl Proof}. Calculate straightforwardly this integral as a sum of the 
integral over $[0,1]$ and the integral over $[1,\infty$:
        Using  equation {1} we come to 
          $$
       \int_0^1
     \left(
     A(t)-\sum_{k<0}\Psi_kt^k-e^{-t}\Psi_0
      \right)
     {dt\over t}= 
       \int_0^1
     \left(
     \sum_{k\geq 0}\Psi_kt^k-e^{-t}\Psi_0
      \right)
     {dt\over t}=
     \sum_{k>0}{\Psi_k\over k}+C_1\Psi_0\,,
       {\rm where}\,\,     
    C_1=\int_0^1(1-e^{-t}){dt\over t}\,,
        $$
and    $$
    \int_1^\infty
     \left(
     A(t)-\sum_{k<0}\Psi_kt^k-e^{-t}\Psi_0
      \right)
     {dt\over t}=
    \int_1^\infty
     A(t){dt\over t}-\sum_{k<0}
    \Psi_k\int_1^\infty t^{k-1}dt-\Psi_0\int_1^\infty e^{-t}{dt\over t}=
     $$
     $$
     \int_1^\infty
     A(t){dt\over t}+\sum_{k<0}
  {\Psi_k\over k}+C_2\Psi_0\,,
  {\rm where}\,\, C_2=-\int_1^\infty e^{-t}{dt\over t}\,.
     $$
Adding these two integrals and subtracting integral (2) we
come to:
       $$
\int_0^\infty
      \left(
     A(t)-\sum_{k<0}\Psi_kt^k-e^{-t}\Psi_0
      \right){dt\over t}
      -
\zeta_A'(0)=
\left(C_1+C_2-C\right)\Psi_0\,.
    \eqno (3)
       $$
  It remains to prove that    $C_1+C_2=C$. 
The nice way to show it is the following:
   Consider
 the function $A(t)=e^{-t}$. Then $\Psi_0=1$ and in equation (4)
 the left hand side is obviously vanished. 
Hence 
          $$
  C_1+C_2-C=0\,,{\rm i.e.}
    \int{(1-e^{-t})dt\over t}-
    \int{e^{-t} dt\over t}=\G'(1)\,.
          $$     
We come to this result without calculations. 


One can formulate the result of the statement as the following identity:
    For an arbitrary function $A(t)$
               $$
{d\over ds}\left({1\over \G(s)}\int_0^\infty t^{s-1}A(t)dt\right)
              \big\vert_{s=0}=
   \int_0^\infty {A(t)-A_-(t)-A_0e^{-t}\over t}dt\,.
               $$
(Left hand side is analytical continuation )
  This formula can be used for  many interesting calculations.
  
\bye 
